Substantial progress on walk subfunctions
Issues with record types seem to be solved, and most functions
can be handled. Lots are a bit of a pain, because the forward
style judgements don't capture all path information by default
(which would create issues with scoping) but it's sometimes
needed to exclude silly cases.

VM_Inst.thy
@@ -4,21 +4,35 @@ theory VM_Inst
 begin
 
 ML \<open>
+structure Let_Atom = struct
+
+fun is_atom t = is_Bound t orelse is_Const t orelse is_Var t orelse is_Free t
+
+fun is_atom_eq t = case try HOLogic.dest_eq t of
+    SOME (x, y) => is_atom x andalso is_atom y
+  | _ => false
+
 val let_atom_simproc = Simplifier.make_simproc @{context} "let_atom"
-  {lhss = [@{term "Let f x"}], proc = fn _ => fn _ => fn ct => let
+  {lhss = [@{term "Let x f"}, @{term "Abbrev (x = y)"}], proc = fn _ => fn _ => fn ct => let
     val t = Thm.term_of ct
-    val (_, xs) = strip_comb t
-    fun is_atom t = is_Bound t orelse is_Const t orelse is_Var t orelse is_Free t
+    val (f, xs) = strip_comb t
+    val f_nm = try (dest_Const #> fst) f
   in
-    if length xs = 2 andalso is_atom (hd xs)
+    if f_nm = SOME @{const_name Let} andalso length xs = 2 andalso is_atom (hd xs)
     then SOME (@{thm Let_def})
+    else if f_nm = SOME @{const_name Abbrev} andalso is_atom_eq (hd xs)
+    then SOME (@{thm Abbrev_def})
     else NONE
   end}
 
-fun let_atom_tac ctxt = simp_tac (put_simpset HOL_basic_ss ctxt addsimprocs [let_atom_simproc])
+fun tac ctxt = simp_tac (put_simpset HOL_basic_ss ctxt addsimprocs [let_atom_simproc])
+
+fun method ctxt = Method.SIMPLE_METHOD (CHANGED (tac ctxt 1))
+
+end
 \<close>
 
-method_setup let_atom = \<open>Scan.succeed (fn ctxt => Method.SIMPLE_METHOD (CHANGED (let_atom_tac ctxt 1)))\<close>
+method_setup let_atom = \<open>Scan.succeed (Let_Atom.method)\<close>
 
 fun(sequential)
   read_const_regs :: "(string set \<times> (string \<Rightarrow> register_value option)) \<Rightarrow> register_value event \<Rightarrow> bool"
@@ -30,8 +44,14 @@ where
 definition
   "const_regs_translate cfg = read_const_regs
     ({''PSTATE'', ''SCR_EL3'', ''HCR_EL2'', ''TCR_EL1'', ''TCR_EL2'', ''TCR_EL3'',
-        ''SCTLR_EL1'', ''SCTLR_EL2'', ''SCTLR_EL3'', ''TTBR0_EL3''
-}, cfg)"
+        ''SCTLR_EL1'', ''SCTLR_EL2'', ''SCTLR_EL3'', ''TTBR0_EL3'', ''TTBR0_EL2'',
+        ''TTBR0_EL1'', ''TTBR1_EL1'', ''TTBR1_EL2'', ''VTCR_EL2'', ''VTTBR_EL2'',
+        ''MAIR_EL1'', ''MAIR_EL2'', ''MAIR_EL3'',
+        ''MPAM3_EL3'', ''_MPAM2_EL2_0_62'', ''_MPAM1_EL1_0_62'',
+        ''MPAM0_EL1'', ''MPAMIDR_EL1'', ''MPAMVPMV_EL2'',
+        ''MPAMVPM0_EL2'', ''MPAMVPM1_EL2'', ''MPAMVPM2_EL2'', ''MPAMVPM3_EL2'',
+        ''MPAMVPM4_EL2'', ''MPAMVPM5_EL2'', ''MPAMVPM6_EL2'', ''MPAMVPM7_EL2'',
+        ''MPAMHCR_EL2''}, cfg)"
 
 definition
   "translate_address_concrete cfg vaddr =
@@ -44,6 +64,9 @@ definition
 abbreviation(input)
   "no_exception m \<equiv> (\<forall>tr e. (m, tr, Exception e) \<notin> Traces)"
 
+abbreviation(input)
+  "monad_semideterm assms m P \<equiv> monad_return_rel assms m m P (=)"
+
 named_theorems no_exception
 
 declare undefined_bitvector_exception[no_exception]
@@ -52,21 +75,48 @@ named_theorems monad_return_rel
 
 named_theorems monad_return_rel_unfold
 
-datatype two = Two_A | Two_B
-
+(* giving this a name helps some automation. we definitely know
+   that we don't know the relation between these vars *)
 definition
-  eq_merge_rel :: "((two list \<Rightarrow> 'a) \<Rightarrow> (two list \<Rightarrow> 'a) \<Rightarrow> 'a) \<Rightarrow> 'a \<Rightarrow> 'a \<Rightarrow> bool"
+  unknown :: "'a \<Rightarrow> 'a \<Rightarrow> bool"
 where
-  "eq_merge_rel f x y = (\<exists>known unknown_l unknown_r. x = f known unknown_l \<and> y = f known unknown_r)"
-
-lemmas eq_merge_relD = eq_merge_rel_def[THEN iffD1]
-lemmas eq_merge_relI = eq_merge_rel_def[THEN iffD2, OF exI, OF exI, OF exI]
+  "unknown a b = True"
 
 lemma monad_return_rel_unknown:
-  "no_exception f \<Longrightarrow> monad_return_rel assms f f (eq_merge_rel (\<lambda>k u. u [])) E"
+  "no_exception f \<Longrightarrow> monad_return_rel assms f f unknown E"
   apply (rule monad_return_rel_rel_weaken[where E=E], rule monad_return_rel_triv, simp_all)
-  apply (auto simp add: eq_merge_rel_def)
+  apply (auto simp add: unknown_def)
   done
+
+lemma unknown_tupleD:
+  "unknown (a, b) (c, d) \<Longrightarrow> unknown a c \<and> unknown b d"
+  by (simp add: unknown_def)
+
+(* this is more silly, avoiding "False" appearing in unification
+   candidates gets away from an annoying capture scenario *)
+definition
+  impossible :: "'a \<Rightarrow> 'a \<Rightarrow> bool"
+where
+  "impossible a b = False"
+
+lemmas monad_return_rel_impossible =
+    FalseE[where P="monad_return_rel assms f g impossible E" for assms f g E]
+
+lemma impossibleE:
+  "impossible a b \<Longrightarrow> P"
+  by (simp add: impossible_def)
+
+(* this one is mostly to make rels easier to type *)
+definition
+  known_unknown_rel :: "('a \<Rightarrow> 'b \<Rightarrow> 'c) \<Rightarrow> 'c \<Rightarrow> 'c \<Rightarrow> bool"
+where
+  "known_unknown_rel f x y = (\<exists>known unknown_l unknown_r. x = f known unknown_l \<and> y = f known unknown_r)"
+
+lemma known_unknown_relE:
+  "known_unknown_rel f x y \<Longrightarrow>
+    (\<And> k u_x u_y. unknown u_x u_y \<Longrightarrow> x = f k u_x \<Longrightarrow> y = f k u_y \<Longrightarrow> P) \<Longrightarrow>
+    P"
+  by (clarsimp simp: known_unknown_rel_def unknown_def)
 
 lemma undefined_bool_exception[no_exception]:
   "no_exception (undefined_bool s)"
@@ -84,6 +134,31 @@ lemma undefined_int_exception[no_exception]:
 lemmas monad_return_rel_undefined_int[monad_return_rel] =
     monad_return_rel_unknown[where f="undefined_int _",
         simplified undefined_int_exception, simplified]
+
+ML \<open>
+fun dest_unknown (Const (@{const_name unknown}, _) $ x $ y) = (x, y)
+  | dest_unknown t = raise TERM ("dest_unknown", [t])
+
+fun conv_schem_apps (Abs (nm, T, t)) = Abs (nm, T, conv_schem_apps t)
+  | conv_schem_apps (f $ x) = if is_Var (head_of f)
+    then Free ("schem_app", fastype_of (f $ x))
+    else conv_schem_apps f $ conv_schem_apps x
+  | conv_schem_apps t = t
+
+fun drop_unknown_tac ctxt = SUBGOAL (fn (t, i) => let
+    val concl = Logic.strip_assums_concl t
+    val concl_bvars = loose_bnos (conv_schem_apps concl) |> Inttab.make_set
+    fun can_drop_atom (Bound i) = not (Inttab.defined concl_bvars i)
+      | can_drop_atom _ = false
+    fun can_drop_unknown t = let
+        val (x, y) = dest_unknown (HOLogic.dest_Trueprop t)
+      in can_drop_atom x andalso can_drop_atom y end
+        handle TERM _ => false
+  in filter_prems_tac ctxt (not o can_drop_unknown) i end)
+\<close>
+
+method_setup drop_unknown = \<open>Scan.succeed () >> (fn _ => fn ctxt =>
+    (Method.SIMPLE_METHOD (drop_unknown_tac ctxt 1)))\<close>
 
 lemma genlistM_exception:
   "(\<And>i. i < n \<Longrightarrow> no_exception (f i)) \<Longrightarrow> no_exception (genlistM f n)"
@@ -135,6 +210,9 @@ lemmas undefined_MemType_exception[no_exception] =
 lemmas undefined_DeviceType_exception[no_exception] =
     undefined_DeviceType_def[THEN def_to_exception, simplified no_exception, simplified]
 
+lemmas monad_return_rel_undefined_DeviceType [monad_return_rel] =
+    undefined_DeviceType_exception[THEN monad_return_rel_unknown]
+
 lemmas undefined_MemAttrHints_exception[no_exception] =
     undefined_MemAttrHints_def[THEN def_to_exception, simplified no_exception bind_no_exception_right simp_thms, simplified]
 
@@ -152,6 +230,9 @@ lemmas monad_return_rel_undefined_MemoryAttributes[monad_return_rel] =
 
 lemmas undefined_MPAMinfo_exception[no_exception] =
     undefined_MPAMinfo_def[THEN def_to_exception, simplified no_exception bind_no_exception_right simp_thms, simplified]
+
+lemmas monad_return_rel_undefined_MPAMinfo [monad_return_rel] =
+    undefined_MPAMinfo_exception[THEN monad_return_rel_unknown]
 
 lemmas undefined_AccessDescriptor_exception[no_exception] =
     undefined_AccessDescriptor_def[THEN def_to_exception, simplified no_exception bind_no_exception_right simp_thms, simplified]
@@ -183,6 +264,7 @@ lemmas undefined_Constraint_exception[no_exception] =
 lemmas monad_return_rel_undefined_Constraint[monad_return_rel] =
     undefined_Constraint_exception[THEN monad_return_rel_unknown]
 
+
 (*
 template for the above
 
@@ -192,6 +274,10 @@ lemmas _exception[no_exception] =
 lemmas monad_return_rel_ [monad_return_rel] =
     _exception[THEN monad_return_rel_unknown]
 *)
+
+lemmas monad_return_rel_undefined_bitvector_unknown =
+    monad_return_rel_unknown[where f="undefined_bitvector _",
+        simplified undefined_bitvector_exception, simplified]
 
 lemma read_reg_exception[no_exception, simp]:
   "no_exception (read_reg r)"
@@ -216,9 +302,11 @@ lemma rel_min_simp[simp]:
   "rel_min P P = P"
   "rel_min P (rel_min P Q) = rel_min P Q"
   "rel_min P (rel_min Q R) = rel_min Q (rel_min P R)"
-  "rel_min P (\<lambda>_ _. False) = P"
-  "rel_min (\<lambda>_ _. False) P = P"
-  by (auto simp add: fun_eq_iff rel_min_def)
+  "rel_min P impossible = P"
+  "rel_min impossible P = P"
+  "rel_min unknown P = unknown"
+  "rel_min P unknown = unknown"
+  by (auto simp add: fun_eq_iff rel_min_def unknown_def impossible_def)
 
 lemma monad_return_rel_if_P:
   "G = G' \<Longrightarrow> (G \<Longrightarrow> monad_return_rel assms f f' P1 E)
@@ -309,6 +397,34 @@ lemma monad_return_rel_return_same_weak:
   "monad_return_rel assms (return x) (return x) (=) E"
   by (rule monad_return_rel_return, simp)
 
+lemma monad_return_rel_return_unit:
+  "monad_return_rel assms (return (x :: unit)) (return y) (=) E"
+  by (rule monad_return_rel_return, simp)
+
+lemmas monad_return_rel_return_unknown = monad_return_rel_return[where P="unknown"]
+
+lemma monad_return_rel_bind_assoc_sym:
+  "monad_return_rel assms
+        (bind (bind f (\<lambda>x. g x)) (\<lambda>y. h y))
+        (bind (bind f' (\<lambda>x. g' x)) (\<lambda>y. h' y)) P E \<Longrightarrow>
+    monad_return_rel assms
+        (bind f (\<lambda>x. bind (g x) (\<lambda>y. h y))) 
+        (bind f' (\<lambda>x. bind (g' x) (\<lambda>y. h' y))) P E"
+  by simp
+
+lemma monad_return_rel_let_as_bind:
+  "monad_return_rel assms (bind (return v) (\<lambda>x. f x)) (bind (return v') (\<lambda>y. g y)) P E \<Longrightarrow>
+    monad_return_rel assms (let x = v in f x) (let y = v' in g y) P E"
+  "monad_return_rel assms (bind (return v) (\<lambda>x. return (j x))) (bind (return v') (\<lambda>y. return (k y))) P E \<Longrightarrow>
+    monad_return_rel assms (return (let x = v in j x)) (return (let y = v' in k y)) P E"
+  by simp_all
+
+lemma monad_return_rel_return_tuple:
+  "monad_return_rel assms (return x) (return x') P E \<Longrightarrow>
+    monad_return_rel assms (return y) (return y') Q E \<Longrightarrow>
+    monad_return_rel assms (return (x, y)) (return (x', y')) (rel_prod P Q) E"
+  by (simp add: monad_return_rel_def)
+
 lemma monad_return_rel_weaken_P:
   "monad_return_rel assms f g P E \<Longrightarrow> (\<And>x y. P x y \<longrightarrow> P' x y) \<Longrightarrow>
     monad_return_rel assms f g P' E"
@@ -318,37 +434,62 @@ lemma rel_min_imp:
   "P x y \<longrightarrow> R \<Longrightarrow> Q x y \<longrightarrow> R \<Longrightarrow> rel_min P Q x y \<longrightarrow> R"
   by (simp add: rel_min_def)
 
-lemmas monad_return_rel_impossible =
-    FalseE[where P="monad_return_rel assms f g (\<lambda>x y. False) E" for assms f g E]
+lemma rel_min_rel_prodD:
+  "rel_min (rel_prod A B) (rel_prod C D) x y \<Longrightarrow> rel_prod (rel_min A C) (rel_min B D) x y"
+  by (auto simp: rel_min_def elim!: rel_prod.cases)
+
+lemmas rel_min_rel_prodDs = 
+    rel_min_rel_prodD[where A="(=)" and B="(=)", simplified prod.rel_eq]
+    rel_min_rel_prodD[where C="(=)" and D="(=)", simplified prod.rel_eq]
+    rel_min_rel_prodD[where A="(=)" and C="(=)", simplified rel_min_simp]
+    rel_min_rel_prodD[where A="(=)" and C="unknown", simplified rel_min_simp]
+    rel_min_rel_prodD[where A="(=)" and C="impossible", simplified rel_min_simp]
+    rel_min_rel_prodD[where A="unknown" and C="(=)", simplified rel_min_simp]
+    rel_min_rel_prodD[where A="unknown" and C="unknown", simplified rel_min_simp]
+    rel_min_rel_prodD[where A="unknown"and C="impossible", simplified rel_min_simp]
+    rel_min_rel_prodD[where A="impossible" and C="(=)", simplified rel_min_simp]
+    rel_min_rel_prodD[where A="impossible" and C="unknown", simplified rel_min_simp]
+    rel_min_rel_prodD[where A="impossible"and C="impossible", simplified rel_min_simp]
 
 lemmas init_monad_return_rel[monad_return_rel] =
     monad_return_rel_assert_exp_P
+    monad_return_rel_assert_exp
     monad_return_rel_if_rel_min
     monad_return_rel_and_boolM
     monad_return_rel_or_boolM
     monad_return_rel_catch_early_return
     monad_return_rel_return_same_weak
-    monad_return_rel_undefined_bitvector
+    monad_return_rel_return_unit
+    monad_return_rel_undefined_bitvector_unknown
+    monad_return_rel_return_tuple
 
-declare bind_assoc[monad_return_rel_unfold]
+lemmas init_return_rel_unfold[monad_return_rel_unfold] =
+    split_paired_all rel_prod_inject case_prod_conv fst_conv snd_conv prod.inject
 
 lemmas monad_return_rel_comb = rel_min_imp conjI impI refl
+        monad_return_rel_bind_assoc_sym
         monad_return_rel_bind monad_return_rel_liftR
+        monad_return_rel_let_as_bind
 
 method read_reg_monad_return_rel =
     ((simp(no_asm) only: const_regs_translate_def)?,
         rule read_reg_monad_return_rel,
         (solves \<open>simp add: register_defs\<close>)?)
 
-method monad_return_rel_step = (determ \<open>intro monad_return_rel monad_return_rel_comb
+method monad_return_rel_step = determ \<open>intro monad_return_rel monad_return_rel_comb
     | rule monad_return_rel
-    | (rule monad_return_rel_impossible, solves \<open>simp only: monad_return_rel_unfold rel_min_simp
-            | let_atom\<close>)
+    | (rule monad_return_rel_impossible,
+        solves \<open>simp only: monad_return_rel_unfold rel_min_simp impossible_def\<close>)
     | simp only: monad_return_rel_unfold rel_min_simp
     | let_atom
+    | drop_unknown
+    | elim conjE conjE[OF unknown_tupleD] exE in_inv_imagep[THEN iffD1, elim_format]
+        known_unknown_relE
+    | erule monad_return_rel_return_unknown rel_min_rel_prodDs[elim_format]
     | (rule monad_return_rel_weaken_P, rule monad_return_rel)
-    | read_reg_monad_return_rel\<close>
-    | (rule monad_return_rel_impossible, solves \<open>clarsimp; simp\<close>))
+    | read_reg_monad_return_rel
+    | (rule monad_return_rel_impossible, solves \<open>clarsimp; simp\<close>)
+  \<close>
 
 method monad_return_rel = monad_return_rel_step+
 
@@ -377,20 +518,25 @@ lemma IsSecureBelowEL3_monad_return_rel[monad_return_rel]:
   done
 
 lemma HighestEL_monad_return_rel[monad_return_rel]:
-  "monad_determ assms (HighestEL ())"
+  "monad_semideterm assms (HighestEL ())
+    (\<lambda>rg rg'. rg = rg' \<and> rg \<in> {EL1, EL2, EL3})"
+  (is "monad_return_rel _ _ _ ?R _")
   apply (simp add: HighestEL_def)
-  apply monad_return_rel
+  apply (rule monad_return_rel_return[where P="?R"]
+    | monad_return_rel_step
+    | simp)+
   done
+
+lemmas EL_exhaust_imp = EL_exhaust_disj[simplified disj_imp, rule_format]
 
 lemma HaveAArch32EL_monad_return_rel[monad_return_rel]:
   "monad_determ assms (HaveAArch32EL el)"
-  using EL_exhaust_disj[of el] monad_return_rel_if_P[monad_return_rel]
   apply (simp add: HaveAArch32EL_def)
   apply (rule
         monad_return_rel_if_rel_min[where ?P1.0="(=)" and ?P2.0="(=)", simplified]
     | monad_return_rel_step
+    | drule(2) EL_exhaust_disj[simplified disj_imp, rule_format]
   )+
-  apply simp
   done
 
 lemma ELStateUsingAArch32K_monad_return_rel[monad_return_rel]:
@@ -449,9 +595,10 @@ lemma AddrTop_monad_return_rel[monad_return_rel]:
   "monad_determ (const_regs_translate cfg) (AddrTop vaddr el)"
   using unat_ELs
   apply (clarsimp simp add: AddrTop_def split del: if_split)
-  apply (monad_return_rel_step
-    | simp only: Let_def
+  apply (rule TrueI
     | (rule monad_return_rel_return[where P="(=)"], clarsimp)
+    | monad_return_rel_step
+    | simp only: Let_def
   )+
   done
 
@@ -467,7 +614,8 @@ declare SCTLR_read__1_def[monad_return_rel_unfold]
 lemma SCTLR_read_monad_return_rel[monad_return_rel]:
   "el \<in> {EL1, EL2, EL3} \<Longrightarrow> monad_determ (const_regs_translate cfg) (SCTLR_read el)"
   apply (simp add: SCTLR_read_def)
-  apply (monad_return_rel | simp)+
+  apply (monad_return_rel)
+  apply (simp add: impossible_def)
   done
 
 lemma AArch64_IsStageOneEnabled_monad_return_rel[monad_return_rel]:
@@ -530,6 +678,7 @@ lemma S2CacheDisabled_monad_return_rel[monad_return_rel]:
   apply (monad_return_rel | clarsimp)+
   done
 
+(*
 lemma eq_merge_rel_apply_update:
   "(\<forall>r x. acc (f x r) = x) \<Longrightarrow>
     eq_merge_rel g_r r r' \<Longrightarrow>
@@ -566,216 +715,545 @@ lemma eq_merge_rel_refl:
 lemma eq_merge_rel_knownD[dest!]:
   "(eq_merge_rel (\<lambda>k u. f k) x y) \<Longrightarrow> (x = y)"
   by (auto simp add: eq_merge_rel_def)
+*)
+
+definition
+  "liftM f m = (bind m (\<lambda>x. return (f x)))"
+
+lemma bind_exception_leftI:
+  "(f, t, Exception e) \<in> Traces \<Longrightarrow> (bind f g, t, Exception e) \<in> Traces"
+  by (induct f arbitrary: t; simp; erule Traces.cases; auto elim!: T.cases)
+
+lemma monad_return_rel_liftM:
+  "monad_return_rel assms (liftM f m) (liftM f m') P E =
+    monad_return_rel assms m m' (\<lambda>x y. P (f x) (f y)) E"
+  apply (rule iffI; subst monad_return_rel_def; clarsimp simp: liftM_def)
+   apply (simp split: monad.split)
+   apply (intro conjI impI allI; clarsimp?;
+     (drule monad_return_relD, ((erule Traces_bindI, simp) | erule bind_exception_leftI)+);
+     simp)
+  apply (simp split: monad.split)
+  apply (auto dest!: bind_Traces_final_cases dest: monad_return_relD)
+  done
+
+lemma rec_to_tuple_coercions:
+  "(\<forall>x. absf (repf x) = x) \<Longrightarrow>
+    bind f (\<lambda>x. g x) = bind (liftM repf f) (\<lambda>x. g (absf x)) \<and>
+    (let x = v in h x) = (let x = repf v in h (absf x)) \<and>
+    (let x = a in j x) = absf (let x = a in repf (j x)) \<and>
+    (if b then v else v') = absf (if b then repf v else repf v') \<and>
+    (unknown v v') = (\<exists>a b. v = absf a \<and> v' = absf b \<and> unknown a b) \<and>
+    (toplevel \<longrightarrow> (monad_return_rel assms f f' (P) (=) =
+        monad_return_rel assms (liftM repf f) (liftM repf f') (\<lambda>x y. P (absf x) (absf y)) (=)))"
+  apply (simp add: monad_return_rel_liftM)
+  apply (simp add: liftM_def unknown_def)
+  apply (auto intro: exI[where x="repf v"] exI[where x="repf v'"])
+  done
+
+lemma liftM_return:
+  "liftM f (return x) = return (f x)"
+  by (simp add: liftM_def)
+
+lemma liftM_bind:
+  "liftM f (bind g (\<lambda>x. h x)) = bind g (\<lambda>x. liftM f (h x))"
+  by (simp add: liftM_def)
+
+lemma liftM_let:
+  "liftM f (let x = v in g x) = (let x = v in liftM f (g x))"
+  by simp
+
+lemmas liftM_if = if_distrib[where f="liftM f" for f]
+
+lemma liftM_liftR:
+  "liftM f (liftR m) = liftR (liftM f m)"
+  apply (simp add: liftM_def liftR_def)
+  apply (induct m, simp_all)
+  apply (simp add: throw_def)
+  done
+
+lemmas rec_to_tuple_extra =
+    liftM_if liftM_return liftM_bind liftM_let liftM_liftR
+
+lemma liftM_unknown:
+  "monad_return_rel assms m m' unknown E \<Longrightarrow>
+    monad_return_rel assms (liftM f m) (liftM f m') unknown E"
+  apply (simp add: liftM_def)
+  apply (erule monad_return_rel_bind)
+  apply (rule monad_return_rel_return)
+  apply (simp add: unknown_def)
+  done
+
+lemma return_rel_via_rep:
+  "monad_return_rel assms (liftM repf f) (liftM repf f') (P) E \<Longrightarrow>
+    monad_return_rel assms f f' (inv_imagep P repf) E"
+  by (simp add: monad_return_rel_liftM inv_imagep_def)
+
+lemma unknown_repD:
+  "unknown x y \<Longrightarrow> unknown (repf x) (repf y)"
+  by (simp add: unknown_def)
+
+ML \<open>
+fun mk_rec_to_tuple_thms ctxt toplevel ty = let
+    val (nm, _) = dest_Type ty
+    val thy = Proof_Context.theory_of ctxt
+    val info = Record.the_info thy (Long_Name.qualifier nm)
+    val (flds, more) = Record.get_extT_fields thy ty
+    val sels = map (fn (nm, ty2) => Const (nm, ty --> ty2)) (flds @ [more])
+    val r = Free ("r", ty)
+    val rep = lambda r (HOLogic.mk_tuple (map (fn sel => sel $ r) sels))
+    val ext_nm = #ext_def info |> Thm.lhs_of |> Thm.term_of |> head_of |> dest_Const |> fst
+    val fld_vs = map (Free o apfst Long_Name.base_name) (flds @ [more])
+    val ext = Const (ext_nm, map type_of fld_vs ---> ty)
+    val abs = HOLogic.tupled_lambda (HOLogic.mk_tuple fld_vs) (list_comb (ext, fld_vs))
+    val top_t = if toplevel then @{cterm True} else @{cterm False}
+    val inst = infer_instantiate ctxt
+        [(("absf", 0), Thm.cterm_of ctxt abs), (("repf", 0), Thm.cterm_of ctxt rep),
+            (("toplevel", 0), top_t)]
+        @{thm rec_to_tuple_coercions}
+    val thm = inst |> simp_tac ctxt 1 |> Seq.hd
+    val t = Var (("t", 0), domain_type (fastype_of abs))
+    val ss_ctxt = put_simpset HOL_basic_ss ctxt
+        addsimps @{thms case_prod_beta} addsimps #select_convs info
+    val sel_apps = map (fn s => s $ (abs $ t)) sels
+        |> map (Thm.cterm_of ctxt #> Simplifier.rewrite ss_ctxt)
+  in thm :: #select_convs info @ #update_convs info @ sel_apps end
+
+fun mk_rec_to_tuple_rules ctxt ty = let
+    val thy = Proof_Context.theory_of ctxt
+    val (nm, _) = dest_Type ty
+    val info = Record.the_info thy (Long_Name.qualifier nm)
+    val (flds, more) = Record.get_extT_fields thy ty
+    val sels = map (fn (nm, ty2) => Const (nm, ty --> ty2)) (flds @ [more])
+    val r = Free ("r", ty)
+    val rep = lambda r (HOLogic.mk_tuple (map (fn sel => sel $ r) sels))
+    val f = infer_instantiate ctxt [(("repf", 0), Thm.cterm_of ctxt rep)]
+  in
+    ([f @{thm return_rel_via_rep}, #equality info], [f @{thm unknown_repD}])
+  end
+
+fun get_tuple_tys1 ctxt t = let
+    val thy = Proof_Context.theory_of ctxt
+    val const_tys = Term.add_consts t [] |> map snd
+    val tys = fold (Term.fold_subtypes (curry (op ::))) const_tys []
+        |> sort_distinct Term_Ord.typ_ord
+  in tys |> filter (can (Record.get_extT_fields thy)) end
+
+fun get_tuple_tys ctxt t = let
+    val thy = Proof_Context.theory_of ctxt
+    val consts = Term.add_consts t []
+    val const_nms = consts |> map fst |> Ord_List.make fast_string_ord
+        |> filter_out (String.isPrefix "HOL")
+    fun shared_consts tms = fold Term.add_consts tms []
+        |> map fst
+        |> Ord_List.make fast_string_ord
+        |> Ord_List.inter fast_string_ord const_nms
+    val cands = consts
+        |> map (snd #> strip_type #> snd)
+        |> sort_distinct Term_Ord.typ_ord
+  in cands
+    |> filter (can (dest_Type #> fst #> Long_Name.qualifier
+        #> Record.the_info thy
+        #> #update_convs #> map Thm.concl_of #> shared_consts #> hd))
+  end
+
+fun rec_via_tuple_tac ctxt = SUBGOAL (fn (t, i) => let
+    val tys = get_tuple_tys1 ctxt t
+    val thms = map (mk_rec_to_tuple_rules ctxt) tys
+    val ss = put_simpset HOL_basic_ss ctxt addsimps @{thms rec_to_tuple_extra}
+        addsimprocs [Record.simproc]
+    val intros = maps fst thms
+    val dests = maps snd thms
+  in (FIRST' [resolve_tac ctxt intros, dresolve_tac ctxt dests,
+    resolve_tac ctxt @{thms monad_return_rel_weaken_P} THEN' resolve_tac ctxt intros]
+    THEN_ALL_NEW simp_tac ss) i end)
+
+fun rec_to_tuple_tac ctxt toplevel = SUBGOAL (fn (t, i) => let
+    val tys = get_tuple_tys ctxt t
+    val thms = maps (mk_rec_to_tuple_thms ctxt toplevel) tys
+  in CHANGED (simp_tac (put_simpset HOL_basic_ss ctxt
+        addsimps thms
+        addsimps @{thms rec_to_tuple_extra prod.collapse}
+        addsimprocs [Record.simproc]) i) end)
+\<close>
+
+method_setup rec_to_tuple = \<open>Scan.lift (Scan.option Parse.name) >> (fn arg => fn ctxt =>
+    Method.SIMPLE_METHOD (rec_to_tuple_tac ctxt (arg = SOME "toplevel") 1))\<close>
+
+method_setup rec_via_tuple = \<open>Scan.succeed () >> (fn _ => fn ctxt =>
+    Method.SIMPLE_METHOD (rec_via_tuple_tac ctxt 1))\<close>
 
 lemma ShortConvertAttrsHints_monad_return_rel[monad_return_rel]:
-  "monad_return_rel (const_regs_translate cfg)
-     (ShortConvertAttrsHints RGN acctype sndstage)
-     (ShortConvertAttrsHints RGN acctype sndstage)
-     (eq_merge_rel
-        (\<lambda>k u. u [] \<lparr>MemAttrHints_attrs := MemAttrHints_attrs (k []),
-               MemAttrHints_hints := MemAttrHints_hints (k [Two_A]),
-               MemAttrHints_transient := MemAttrHints_transient (k [Two_B])\<rparr>)) (=)"
-  (is "monad_return_rel _ _ _ ?R _")
-  using word_unat.univ[THEN eqset_imp_iff, where x=RGN, simplified]
-  apply (simp add: ShortConvertAttrsHints_def unats_def lessThan_def[symmetric]
-        lessThan_nat_numeral lessThan_Suc Let_def[where s=RGN]
-        cong: if_cong)
-  apply (monad_return_rel
-    | rule MemAttrs_merge eq_merge_rel_refl monad_return_rel_return_merge
-    | assumption)+
+  "monad_determ (const_regs_translate cfg)
+     (ShortConvertAttrsHints RGN acctype sndstage)"
+
+  unfolding ShortConvertAttrsHints_def
+  apply (rule monad_return_rel_weaken_P)
+  apply ((monad_return_rel
+    | (rule liftM_unknown, rule monad_return_rel)
+    | rec_via_tuple
+    | rule monad_return_rel_return_tuple monad_return_rel_let_as_bind
+  )+)[1]
   apply simp
-thm MemAttrs_merge
+  done
 
+declare UNKNOWN_bits_def[monad_return_rel_unfold] UNKNOWN_integer_def[monad_return_rel_unfold]
+    UNKNOWN_boolean_def[monad_return_rel_unfold]
+
+lemma known_unknown_simpleI:
+  "(\<exists>a b. f x a = x \<and> f x b = y) \<Longrightarrow> known_unknown_rel f x y"
+  apply (clarsimp simp: known_unknown_rel_def)
+  apply metis
+  done
+
+lemma AArch64_AccessFlagFault_monad_return_rel[monad_return_rel]:
+  "monad_semideterm assms
+    (AArch64_AccessFlagFault ipaddress level acctype iswrite sndstage s2fs1walk)
+    (known_unknown_rel (\<lambda>r (x, y, z, d). r \<lparr> FaultRecord_debugmoe := x, FaultRecord_errortype := y,
+        FaultRecord_extflag := z, FaultRecord_domain := d \<rparr> ))"
+  apply (simp add: AArch64_AccessFlagFault_def AArch64_CreateFaultRecord_def)
+  apply (monad_return_rel | rec_via_tuple)+
+  apply (clarsimp intro!: known_unknown_simpleI)
+  apply (intro exI conjI FaultRecord.equality, simp_all)
+  done
+
+lemma AArch64_AddressSizeFault_monad_return_rel[monad_return_rel]:
+  "monad_semideterm assms
+    (AArch64_AddressSizeFault ipaddress level acctype iswrite sndstage s2fs1walk)
+    (known_unknown_rel (\<lambda>r (x, y, z, d). r \<lparr> FaultRecord_debugmoe := x, FaultRecord_errortype := y,
+        FaultRecord_extflag := z, FaultRecord_domain := d \<rparr> ))"
+  apply (simp add: AArch64_AddressSizeFault_def AArch64_CreateFaultRecord_def)
   apply monad_return_rel
-apply (rule monad_return_rel_return_merge, (rule MemAttrs_merge eq_merge_rel_refl | assumption)+)
+  apply (rule monad_return_rel_return)
+  apply (clarsimp intro!: known_unknown_simpleI simp only: split_paired_Ex)
+  apply (intro exI conjI FaultRecord.equality, simp_all)
+  done
 
-  apply (monad_return_rel
-    | rule to_eq_merge_rel
-    | ((rule
-    return_eq_after_update
-[where acc="MemAttrHints_hints" and f="\<lambda>x. MemAttrHints_hints_update (\<lambda>_. x)", simplified]
-    return_eq_after_update[where acc="MemAttrHints_attrs" and f="\<lambda>x. MemAttrHints_attrs_update (\<lambda>_. x)", simplified]
-)+, rule
-    monad_return_rel_return[where P="\<lambda>_ _. True", OF TrueI]
-)
-)+
+lemma AArch64_NoFault_monad_return_rel[monad_return_rel]:
+  "monad_semideterm assms
+    (AArch64_NoFault x)
+    (known_unknown_rel (\<lambda>r (x, y, z, a, b, c, d).
+        r \<lparr> FaultRecord_debugmoe := x, FaultRecord_errortype := y,
+        FaultRecord_extflag := z, FaultRecord_domain := d, FaultRecord_level := a,
+        FaultRecord_ipaddress := b, FaultRecord_write := c \<rparr> ))"
+  apply (simp add: AArch64_NoFault_def AArch64_CreateFaultRecord_def)
+  apply monad_return_rel
+  apply (rule monad_return_rel_return)
+  apply (clarsimp intro!: known_unknown_simpleI)
+  apply (intro exI conjI FaultRecord.equality, simp_all)
+  done
 
-apply (rule to_eq_merge_rel)
-apply (rule to_eq_merge_rel)
-apply (monad_return_rel)
+declare HaveMPAMExt_def[monad_return_rel_unfold]
 
-apply ((rule
-    return_eq_after_update[where acc="MemAttrHints_hints" and f="\<lambda>x. MemAttrHints_hints_update (\<lambda>_. x)", simplified]
-    return_eq_after_update[where acc="MemAttrHints_attrs" and f="\<lambda>x. MemAttrHints_attrs_update (\<lambda>_. x)", simplified]
-)+, rule
-    monad_return_rel_return[where P="\<lambda>_ _. True", OF TrueI]
-)
+lemma MPAM2_EL2_read_monad_return_rel[monad_return_rel]:
+  "monad_determ (const_regs_translate cfg) (MPAM2_EL2_read u)"
+  apply (simp add: MPAM2_EL2_read_def)
+  apply monad_return_rel
+  apply (rule monad_return_rel_return)
+  apply (simp add: set_slice_def update_subrange_vec_dec_def)
+  apply (rule word_eqI, simp add: test_bit_word_update)
+  done
 
+lemma unknown_eq_at_bits:
+  "unknown x y \<Longrightarrow> eq_at_bits {} x y"
+  by (simp add: eq_at_bits_def)
 
-  apply (monad_return_rel
-| rule
-    monad_return_rel_let_via_bind
-    to_eq_merge_rel
+lemmas monad_return_rel_return_eq_at_bits = monad_return_rel_return[where P="eq_at_bits S" for S]
+
+lemma return_word_update_lemma:
+  assumes eq: "eq_at_bits S x x'"
+   and extra: "j = i + size y - 1" "j < size x" "0 < size y"
+  shows "monad_return_rel assms (return (word_update x i j y)) (return (word_update x' i j y))
+    (eq_at_bits (S \<union> {nat i ..< nat j + 1})) E"
+  using eq extra
+  by (auto simp: eq_at_bits_def test_bit_word_update intro!: monad_return_rel_return)
+
+lemma MPAM1_EL1_read_monad_return_rel[monad_return_rel]:
+  "monad_determ (const_regs_translate cfg) (MPAM1_EL1_read u)"
+  apply (simp add: MPAM1_EL1_read_def)
+  apply (simp only: set_slice_def update_subrange_vec_dec_def)
+  apply (rule monad_return_rel_weaken_P)
+   apply (monad_return_rel
+     | (rule return_word_update_lemma, (assumption | erule unknown_eq_at_bits),
+         simp+)[1]
+     | erule monad_return_rel_return_eq_at_bits
+   )+
+  apply (auto dest: eq_at_bits_complete)
+  done
+
+lemma MPAMisEnabled_monad_return_rel[monad_return_rel]:
+  "monad_determ (const_regs_translate cfg) (MPAMisEnabled u)"
+  apply (simp add: MPAMisEnabled_def)
+  apply ((rule monad_return_rel_impossible, solves \<open>simp\<close>)
+    | monad_return_rel_step)+
+  apply (simp add: impossible_def)
+  done
+
+lemma EL2Enabled_monad_return_rel[monad_return_rel]:
+  "monad_determ (const_regs_translate cfg) (EL2Enabled u)"
+  apply (simp add: EL2Enabled_def)
+  apply monad_return_rel
+  done
+
+lemma getMPAM_PARTID_monad_return_rel[monad_return_rel]:
+  "MPAMn \<in> {0, 1, 2, 3} \<Longrightarrow> monad_determ (const_regs_translate cfg) (getMPAM_PARTID MPAMn in_d)"
+  apply (simp only: getMPAM_PARTID_def Let_def[where s=MPAMn] mem_simps)
+  apply (elim disjE; simp cong: if_cong)
+     apply monad_return_rel
+  done
+
+lemma MPAMisVirtual_monad_return_rel[monad_return_rel]:
+  "monad_determ (const_regs_translate cfg) (MPAMisVirtual MPAMn)"
+  apply (simp add: MPAMisVirtual_def)
+  apply monad_return_rel
+  done
+
+lemma mapvpmw_monad_return_rel[monad_return_rel]:
+  "monad_determ (const_regs_translate cfg) (mapvpmw partid)"
+  apply (simp add: mapvpmw_def)
+  apply monad_return_rel
+  done
+
+lemma MAP_vPARTID_monad_return_rel[monad_return_rel]:
+  "monad_determ (const_regs_translate cfg) (MAP_vPARTID partid)"
+  apply (simp add: MAP_vPARTID_def)
+  apply monad_return_rel
+  apply clarsimp
+  apply monad_return_rel
+  done
+
+lemma genPARTID_monad_return_rel[monad_return_rel]:
+  "MPAMn \<in> {0, 1, 2, 3} \<Longrightarrow> monad_determ (const_regs_translate cfg) (genPARTID MPAMn in_d)"
+  apply (simp add: genPARTID_def)
+  apply monad_return_rel
+  apply (simp only: mem_simps simp_thms)
+  apply monad_return_rel
+  done
+
+lemma getMPAM_PMG_monad_return_rel[monad_return_rel]:
+  "el \<in> {0, 1, 2, 3} \<Longrightarrow> monad_determ (const_regs_translate cfg) (getMPAM_PMG el in_d)"
+  apply (simp add: getMPAM_PMG_def cong: if_cong)
+  apply ((rule monad_return_rel_impossible, solves \<open>simp\<close>)
+    | monad_return_rel_step
+    | simp add: impossible_def)+
+  done
+
+lemma genPMG_monad_return_rel[monad_return_rel]:
+  "el \<in> {0, 1, 2, 3} \<Longrightarrow> monad_determ (const_regs_translate cfg) (genPMG el in_d partid_err)"
+  apply (simp add: genPMG_def)
+  apply (monad_return_rel | simp)+
+  done
+
+lemma genMPAM_monad_return_rel[monad_return_rel]:
+  "el \<in> {0, 1, 2, 3} \<Longrightarrow> monad_determ (const_regs_translate cfg) (genMPAM el in_d secure)"
+  apply (simp only: genMPAM_def Let_def[where s="if _ then _ else el"])
+  apply (monad_return_rel | rec_via_tuple | simp)+
+  done
+
+lemma DefaultMPAMinfo_monad_return_rel[monad_return_rel]:
+  "monad_determ (const_regs_translate cfg) (DefaultMPAMinfo sec)"
+  apply (simp add: DefaultMPAMinfo_def)
+  apply (monad_return_rel | rec_via_tuple)+
+  done
+
+lemma GenMPAMcurEL_monad_return_rel[monad_return_rel]:
+  "monad_determ (const_regs_translate cfg) (GenMPAMcurEL inD)"
+  apply (simp add: GenMPAMcurEL_def)
+  apply monad_return_rel
+    apply (rule word_uint.Rep[THEN subsetD[rotated]])
+    apply (simp add: uints_unats unats_def lessThan_def[symmetric]
+        lessThan_nat_numeral lessThan_Suc)
+   apply monad_return_rel
+  done
+
+lemma CreateAccessDescriptorPTW_monad_return_rel[monad_return_rel]:
+  "monad_determ (const_regs_translate cfg) (CreateAccessDescriptorPTW acctype sndstage s2fs1walk level)"
+  apply (simp add: CreateAccessDescriptorPTW_def)
+  apply (monad_return_rel | rec_via_tuple)+
+  done
+
+lemmas more_unknowns[monad_return_rel_unfold] =
+  UNKNOWN_DeviceType_def UNKNOWN_MemAttrHints_def UNKNOWN_bits_def
+
+lemma rel_min_inv_image[simp, monad_return_rel_unfold]:
+  "rel_min (inv_imagep A f) (inv_imagep B f) x y = rel_min A B (f x) (f y)"
+  by (auto simp: rel_min_def)
+
+lemma unknownI:
+  "unknown a b"
+  by (simp add: unknown_def)
+
+lemma MemAttrDefaults_monad_return_rel[monad_return_rel]:
+  "monad_return_rel assms
+    (MemAttrDefaults x)
+    (MemAttrDefaults x)
+    (\<lambda>r r'. \<exists>inn out fgen dev. r = r' \<lparr>MemoryAttributes_inner := inn, MemoryAttributes_outer := out, MemoryAttributes_readtagfaulttgen := fgen, MemoryAttributes_device := dev\<rparr> 
+        \<and> unknown (inn, out, fgen, dev) (MemoryAttributes_inner r', MemoryAttributes_outer r', MemoryAttributes_readtagfaulttgen r', MemoryAttributes_device r')) (=)"
+  apply (simp add: MemAttrDefaults_def split del: if_split)
+  apply (rule monad_return_rel_weaken_P)
+   apply (monad_return_rel
+    | (rule liftM_unknown, rule monad_return_rel)
+    | rule monad_return_rel_let_Abbrev
+    | simp only: if_distrib[where f=return]
+    | rec_via_tuple
   )+
+  apply (intro impI exI conjI unknownI MemoryAttributes.equality, simp_all)
+  done
 
-apply ((rule
-    return_eq_after_update[where acc="MemAttrHints_hints" and f="\<lambda>x. MemAttrHints_hints_update (\<lambda>_. x)", simplified]
-    return_eq_after_update[where acc="MemAttrHints_attrs" and f="\<lambda>x. MemAttrHints_attrs_update (\<lambda>_. x)", simplified]
-)+, rule
-    monad_return_rel_return[where P="\<lambda>_ _. True", OF TrueI]
-)
-
-  apply (monad_return_rel
-| rule
-    monad_return_rel_let_via_bind
-    to_eq_merge_rel
-  )+
-
-apply ((rule
-    return_eq_after_update[where acc="MemAttrHints_hints" and f="\<lambda>x. MemAttrHints_hints_update (\<lambda>_. x)", simplified]
-    return_eq_after_update[where acc="MemAttrHints_attrs" and f="\<lambda>x. MemAttrHints_attrs_update (\<lambda>_. x)", simplified]
-)+, rule
-    monad_return_rel_return[where P="\<lambda>_ _. True", OF TrueI]
-)
-
-  apply (monad_return_rel
-| rule
-    monad_return_rel_let_via_bind
-    to_eq_merge_rel
-  )+
-
-apply ((rule
-    return_eq_after_update[where acc="MemAttrHints_hints" and f="\<lambda>x. MemAttrHints_hints_update (\<lambda>_. x)", simplified]
-    return_eq_after_update[where acc="MemAttrHints_attrs" and f="\<lambda>x. MemAttrHints_attrs_update (\<lambda>_. x)", simplified]
-)+, rule
-    monad_return_rel_return[where P="\<lambda>_ _. True", OF TrueI]
-)
-
-
-  apply (
- rule
-    monad_return_rel_let_via_bind
-    to_eq_merge_rel
-  )+
-
-apply (monad_return_rel_step)
-apply (monad_return_rel_step)
-
-apply (rule
-    monad_return_rel_return[where P="\<lambda>_ _. True", OF TrueI]
-)
-
-apply ( monad_return_rel
-  | rule
-    return_eq_after_update[where acc="MemAttrHints_attrs" and f="\<lambda>x. MemAttrHints_attrs_update (\<lambda>_. x)", simplified]
-    return_eq_after_update[where acc="MemAttrHints_hints" and f="\<lambda>x. MemAttrHints_hints_update (\<lambda>_. x)", simplified]
-
-    monad_return_rel_let_via_bind
-    to_eq_merge_rel
-  | simp only:
-  | rule monad_return_rel_return[where P="\<lambda>_ _. True", OF TrueI]
-)+
-
-
-apply (monad_return_rel)
-apply ( rule
-    return_eq_after_update[where acc="MemAttrHints_attrs" and f="\<lambda>x. MemAttrHints_attrs_update (\<lambda>_. x)", simplified]
-    return_eq_after_update[where acc="MemAttrHints_hints" and f="\<lambda>x. MemAttrHints_hints_update (\<lambda>_. x)", simplified]
-
-    monad_return_rel_let_via_bind
-    to_eq_merge_rel
-  | simp only:
-)+
-apply (monad_return_rel)
-
-apply ( rule
-    return_eq_after_update[where acc="MemAttrHints_attrs" and f="\<lambda>x. MemAttrHints_attrs_update (\<lambda>_. x)", simplified]
-    return_eq_after_update[where acc="MemAttrHints_hints" and f="\<lambda>x. MemAttrHints_hints_update (\<lambda>_. x)", simplified]
-
-    monad_return_rel_let_via_bind
-    to_eq_merge_rel
-  | simp only:
-)+
-
-
-apply (rule
-    monad_return_rel_return[where P="\<lambda>_ _. True", OF TrueI]
-)
-
-apply ( rule
-    return_eq_after_update[where acc="MemAttrHints_attrs" and f="\<lambda>x. MemAttrHints_attrs_update (\<lambda>_. x)", simplified]
-    return_eq_after_update[where acc="MemAttrHints_hints" and f="\<lambda>x. MemAttrHints_hints_update (\<lambda>_. x)", simplified]
-
-    monad_return_rel_let_via_bind
-    to_eq_merge_rel
-  | simp only:
-)+
-
-
-thm let_double_refold
-
-apply simp
-apply simp
+lemma monad_return_rel_liftM_intro:
+  "monad_return_rel assms m m' P E \<Longrightarrow>
+    monad_return_rel assms (liftM f m) (liftM g m') (\<lambda>x y. \<exists>x' y'. x = f x' \<and> y = g y' \<and> P x' y') E"
+  apply (simp add: liftM_def)
+  apply (erule monad_return_rel_bind)
+  apply (rule monad_return_rel_return)
+  apply auto
   done
 
 lemma WalkAttrDecode_monad_return_rel[monad_return_rel]:
-  "monad_determ (const_regs_translate cfg)
-  (WalkAttrDecode SH ORGN IRGN sndstage)"
-  apply (simp add: WalkAttrDecode_def)
+  "monad_semideterm (const_regs_translate cfg)
+    (WalkAttrDecode SH ORGN IRGN sndstage)
+    (\<lambda>r r'. \<exists>fgen dev. r = r' \<lparr>MemoryAttributes_readtagfaulttgen := fgen, MemoryAttributes_device := dev\<rparr> 
+        \<and> unknown (fgen, dev) (MemoryAttributes_readtagfaulttgen r', MemoryAttributes_device r'))"
+  apply (simp add: WalkAttrDecode_def MemAttrDefaults_def)
+  apply (rule monad_return_rel_weaken_P)
+
+  apply (monad_return_rel
+    | rule monad_return_rel_let_Abbrev
+    | simp only: if_distrib[where f=return]
+    | rec_via_tuple
+)+
+  apply (intro impI exI conjI unknownI MemoryAttributes.equality, simp_all)
+  done
+
+declare MAIR_read__1_def[monad_return_rel_unfold]
+
+lemma MAIR_read_monad_return_rel[monad_return_rel]:
+  "el \<in> {EL1, EL2, EL3} \<Longrightarrow> monad_determ (const_regs_translate cfg) (MAIR_read el)"
+  apply (simp add: MAIR_read_def)
   apply monad_return_rel
+  apply (simp add: impossible_def)
+  done
+
+declare Unreachable_def[monad_return_rel_unfold]
+
+lemma LongConvertAttrsHints_monad_return_rel[monad_return_rel]:
+  "monad_semideterm (const_regs_translate cfg)
+    (LongConvertAttrsHints attr acctype)
+    (known_unknown_rel (\<lambda>r x. r \<lparr> MemAttrHints_transient := x  \<rparr> ))"
+  apply (simp add: LongConvertAttrsHints_def)
+  apply (rule monad_return_rel_weaken_P)
+  apply (monad_return_rel
+    | simp only: if_distrib[where f=return]
+    | rec_via_tuple
+    | rule known_unknown_simpleI exI)+
+  done
+
+lemma assert_exp_False:
+  "assert_exp False s = Fail s"
+  by (simp add: assert_exp_def)
+
+lemmas monad_return_rel_return_spec =
+    monad_return_rel_return[where x=z and y=z and P="\<lambda>x y. x = z \<and> y = z" for z]
+
+lemma monad_return_rel_Fail[monad_return_rel]:
+  "monad_return_rel assms (Fail s) (Fail s') impossible E"
+  by (simp add: monad_return_rel_def)
+
+lemmas rel_minE = rel_min_def[THEN iffD1, THEN disjE]
+
+lemma monad_return_rel_rel_min_split:
+  "rel_min P Q x y \<Longrightarrow>
+    (P x y \<Longrightarrow> monad_return_rel assms f g R E) \<Longrightarrow>
+    (Q x y \<Longrightarrow> monad_return_rel assms f g S E) \<Longrightarrow>
+    monad_return_rel assms f g (rel_min R S) E"
+  by (auto simp: rel_min_def elim!: monad_return_rel_weaken_P)
+
+lemma AArch64_S1AttrDecode_monad_return_rel[monad_return_rel]:
+  "monad_semideterm (const_regs_translate cfg)
+    (AArch64_S1AttrDecode SH attr acctype)
+    (known_unknown_rel (\<lambda>r (inn, out, fgen, dev). r \<lparr> MemoryAttributes_inner := inn,
+        MemoryAttributes_outer := out, MemoryAttributes_readtagfaulttgen := fgen, MemoryAttributes_device := dev\<rparr>))"
+  apply (simp add: AArch64_S1AttrDecode_def)
+  apply (simp only: ConstrainUnpredictableBits_def[where which=Unpredictable_RESMAIR, simplified]
+                    Unreachable_def assert_exp_False bind.simps Let_def)
+  apply (rule monad_return_rel_weaken_P)
+   apply ((rule monad_return_rel_return_spec[where z=MemType_Device]
+        | monad_return_rel_step
+        | rec_via_tuple)+)
+  apply (erule monad_return_rel_rel_min_split;
+    simp add: MemAttrDefaults_def liftM_bind liftM_return split del: if_split)
+   apply (monad_return_rel
+    | simp only: if_distrib[where f=return]
+    | rec_via_tuple
+    | (rule known_unknown_simpleI; simp; intro exI conjI MemoryAttributes.equality; simp)
+    | drule rel_min_rel_prodD
+  )+
+  done
+
+lemma S2ConvertAttrsHints_monad_return_rel[monad_return_rel]:
+  "monad_determ assms (S2ConvertAttrsHints attr acctype)"
+  apply (simp add: S2ConvertAttrsHints_def)
+  apply (rule monad_return_rel_weaken_P)
+   apply (monad_return_rel | rec_via_tuple)+
+  done
+
+declare UNKNOWN_MemoryAttributes_def[monad_return_rel_unfold]
+
+lemma S2AttrDecode_monad_return_rel[monad_return_rel]:
+  "monad_semideterm (const_regs_translate cfg)
+    (S2AttrDecode SH attr acctype)
+    (known_unknown_rel (\<lambda>r (inn, out, fgen, dev). r \<lparr> MemoryAttributes_inner := inn,
+        MemoryAttributes_outer := out, MemoryAttributes_readtagfaulttgen := fgen, MemoryAttributes_device := dev\<rparr>))"
+  apply (simp add: S2AttrDecode_def)
+  apply (simp only: bind_assoc[symmetric] mem_simps, intro monad_return_rel_bind
+                    assert_exp_False bind.simps)
+    apply ((rule monad_return_rel_return_spec[where z=MemType_Device]
+        | monad_return_rel_step
+        | rec_via_tuple)+)[2]
+  apply simp
+  (* OK, this is interesting. The attributes of this are set unspecified in
+     a very unspecified way, which was probably not intended. *)
+  sorry
 
 
 text {*
-lemma AArch64_NoFault_monad_return_rel[monad_return_rel]:
-  "monad_return_rel assms (AArch64_NoFault x) (AArch64_NoFault y)
-    (\<lambda>ft ft'. FaultRecord_statuscode ft = Fault_None \<and> FaultRecord_statuscode ft' = Fault_None) (=)"
-  apply (simp add: AArch64_NoFault_def AArch64_CreateFaultRecord_def
-                   UNKNOWN_bits_def UNKNOWN_integer_def UNKNOWN_boolean_def)
-  apply (monad_return_rel
-    | rule monad_return_rel_bind[OF monad_return_rel_undefined_FaultRecord]
-    | simp)+
-  done
-
-lemma monad_return_rel_let_binop_shuffle:
-  "monad_return_rel assms (let x = x; y = y in g (f x y)) (let x = x'; y = y' in g' (f x y)) Q E \<Longrightarrow>
-    monad_return_rel assms (let z = f x y in g z) (let z = f x' y' in g' z) Q E"
-  by simp
-
-
-
 lemma AArch64_TranslationTableWalk_monad_return_rel[monad_return_rel]:
   "monad_determ (const_regs_translate cfg)
     (AArch64_TranslationTableWalk ipaddress vaddr acctype iswrite sndstage s2fs sz)"
   using [[simproc del: let_simp]]
-  apply (simp only: AArch64_TranslationTableWalk_def tlb_disabled)
+  apply (simp only: AArch64_TranslationTableWalk_def tlb_disabled bind_assoc[symmetric] if_simps)
   apply (monad_return_rel
-    | rule
-        monad_return_rel_let_Abbrev
-        monad_return_rel_if_P
-        monad_return_rel_bind[where P="\<lambda>_ (_ :: unit). True"]
+    | rule monad_return_rel_let_Abbrev monad_return_rel_let_as_bind
+    | simp only: liftR_bind_split
+    | (rule liftM_unknown, rule monad_return_rel)
+    | erule monad_return_rel_return_unknown monad_return_rel_return_eq_at_bits rel_min_rel_prodDs[elim_format]
+  )+
+
+  apply (drop_unknown | rec_via_tuple)+
+
+  apply (monad_return_rel
+    | rule monad_return_rel_let_Abbrev monad_return_rel_return_tuple monad_return_rel_let_as_bind
+    | simp only: liftR_bind_split
+    | erule monad_return_rel_return_unknown monad_return_rel_return_eq_at_bits rel_min_rel_prodDs[elim_format]
+    | drop_unknown | rec_via_tuple
+  )+
+
+apply rec_via_tuple
+
+apply rec_via_tuple
+
+apply rec_via_tuple
+
+apply monad_return_rel
+
+apply rec_via_tuple
+
+
+  apply rec_to_tuple
+
+  apply (monad_return_rel
+    | rule monad_return_rel_let_Abbrev monad_return_rel_return_tuple
     | simp only: liftR_bind_split
   )+
-
-  apply (monad_return_rel
-    | rule
-        monad_return_rel_assert_exp
-        monad_return_rel_bind[where P="(=) :: bool \<Rightarrow> _"]
-        monad_return_rel_bind[where P="(=)", where f="if tlb_enabled then _ else _"]
-        monad_return_rel_let_Abbrev
-    | simp only: if_simps bind_return
-  )+
-
-
-apply (let_atom
-  | rule
-    monad_return_rel_let_binop_shuffle[where f="\<lambda>x y. y \<lparr> AddressDescriptor_memattrs := x \<rparr>"]
-    monad_return_rel_let_binop_shuffle[where f="\<lambda>x y. y \<lparr> MemoryAttributes_memtype := x \<rparr>"]
-        monad_return_rel_let_Abbrev
-monad_return_rel_acc_disagree[where acc="AddressDescriptor_memattrs"]
-   monad_return_rel_if_P[where G="\<not> sndstage", THEN monad_return_rel_bind_eq]
-)+
-
-
 
   apply (monad_return_rel
     | rule
